

pset 2*

Jaden Lee

Thursday, 1/29/26

<https://yale.instructure.com/courses/113840/assignments/558950>

1 Problem 1

Show how to come to the conclusion v given the following premises. Show which rule of inference you used at each step and which premises and/or previous conclusions you applied them to.

$p \vee \neg q \vee r$
$p \rightarrow s$
$s \rightarrow v$
$\neg q \rightarrow \neg u$
u
$r \rightarrow v$

1.1 solution

we are given $u=\text{true}$. from this, using negation, we can derive that $\neg u$ is false. From this we can further derive that, because $\neg q \rightarrow \neg u$ is true and since $\neg u$ is false, we are forced to conclude that $\neg q$ is also false.

In other words, if we were to entertain that $\neg q$ is true while knowing $\neg u$ is false, that would result in us concluding that the given predicate $\neg q \rightarrow \neg u$ is not true, which is not the case.

*made in Overleaf

From here, we arrive at the rule that $p \vee \neg q \vee r$. However, since we know $\neg q$ to be false, we must assume that either r is true or p is true. In other words, we know that $r \vee p$ must be true.

From here, we may consider the case that p is true. Since we are given the rule that $p \rightarrow s$, to abide by this rule in this scenario s is true. From this, we are also given that $s \rightarrow v$, so to abide by *that* rule, v must also be true.

Now let us consider the other case. In the case that r is true, we are given the rule that $r \rightarrow v$. Abiding by this given predicate, we can arrive at the conclusion that v must also be true.

As demonstrated, regardless of whether either r or p is true (or both), it can be concluded that v must be true from the above conclusions. if one were to demonstrate this in a predicate-formative manner, we could say that the statement

$$(p \vee r) \rightarrow v$$

is true, thus making v true.

2 Problem 2

You meet four people on the Island of Knights and Knaves. Given the following statements they make, determine for each individual whether they are a knight or a knave. Show your reasoning. (Knights' statements are always true and knaves' statements are always false, but consider each utterance as a single (possibly compound) statement, so if a knave's statement is a conjunction, then at least one of the conjuncts must be false, but other conjuncts may be true).

- A: I am a knight and C is a knave.
- B: A is a knave.
- C: There is only one knight and it is not me.
- D: A and myself are the only knights among us.

2.1 solution

Let us assume that B is a knight. We can conclude from this that A is a knave. As A says that A is a knight and C is a knave, we can further derive that C is a knight. However, C states that there is only one knight and it is not C. We have arrived at a contradicting statement. C, despite being a knight in this scenario, is saying something that conflicts with our established conclusions.

However, let us entertain A's compound statement, that A being a knight is false, but C being a knave is true (we cannot assume the inverse in this scenario). We can conclude that there is either multiple knights or that C is not a knight, or both. Seeing as C must be a knave, the only possible true predicate in this compound statement is that there are multiple knights.

We thus arrive at the conclusion that D must be a knight. However, D says a compound statement that D *AND* A are knights. Since both of these things must be true, and that in this scenario, A must be a knave due to B's assumed knighthood and statements, we are forced to conclude that B cannot be a knight.

Now, let us assume that B is a knave. We can conclude that A is a knight. A declares themselves a knight (true) and C is a knave. C says there is only one knight, and it is not C. The latter half already having been proven true, we can turn to the former and say that D is the only remaining option as the other knight. D's statement agrees with this, saying A and D are the only knights; a conclusion that reasons well with our arrived conclusion.

Thus, A and D are knights

3 Problem 3

Let P be the set of players, T be the set of professional teams, and C be the set of college teams. Let $M(x, y)$ be the predicate "player x plays for pro team y " and $N(x, y)$ be the predicate "player x played for college team y "

Write each of the following in predicate logic. Be sure to indicate the domain of each quantified variable using P, T , or C . Assume that the specific nouns mentioned are members of the appropriate sets.

- No player played for Harvard. [note: Harvard is a college team]
- Every player who plays for Golden State played for Virginia. [note: Golden State is a pro team and Virginia is a college team]

- Some player didn't play for any college team.
- For every college team, there is a player who played for them and plays for a pro team.
- Every player played for a unique college team. [note: use logical connectives, the predicates defined above, and the two standard quantifiers \forall and \exists ; you may also use $=$ (which is really a two-place predicate written using infix notation rather than function notation, so $x = y$ can be thought of as the predicate $= (x, y)$ meaning " x and y are the same element")]

3.1 solution

statement	statement	domain
No player played for Harvard. [note: Harvard is a college team]	$\neg\forall x[N(x, \text{harvard})]$	$x \in P$
Every player who plays for Golden State played for Virginia. [note: Golden State is a pro team and Virginia is a college team]	$\forall x[M(x, \text{GoldenState}) \rightarrow N(x, \text{Virginia})]$	$x \in P$
Some player didn't play for any college team.	$\exists x\forall y[N(x, y)]$	$x \in P, y \in C$
For every college team, there is a player who played for them and plays for a pro team.	$\exists x\forall y\exists z[N(x, y) \wedge M(x, z)]$	$x \in P, y \in C, z \in T$
Every player played for a unique college team. [note: use logical connectives, the predicates defined above, and the two standard quantifiers \forall and \exists ; you may also use $=$ (which is really a two-place predicate written using infix notation rather than function notation, so $x = y$ can be thought of as the predicate $=(x, y)$ meaning “ x and y are the same element”)]	$\forall x\exists y\exists z[(N(x, y) \wedge \neg N(z, y)) \wedge \neg(x = z)]$	$x \in P, z \in P, y \in C$

note that this table notation is for ease of reading